src/ocaml/extraction/BinNat.mli
@@ -5,6 +5,10 @@ open Decimal
 
 module N :
  sig
+  val succ_double : coq_N -> coq_N
+
+  val double : coq_N -> coq_N
+
   val succ : coq_N -> coq_N
 
   val add : coq_N -> coq_N -> coq_N
@@ -17,7 +21,19 @@ module N :
 
   val eqb : coq_N -> coq_N -> bool
 
+  val leb : coq_N -> coq_N -> bool
+
   val ltb : coq_N -> coq_N -> bool
+
+  val even : coq_N -> bool
+
+  val odd : coq_N -> bool
+
+  val pos_div_eucl : positive -> coq_N -> coq_N * coq_N
+
+  val div_eucl : coq_N -> coq_N -> coq_N * coq_N
+
+  val div : coq_N -> coq_N -> coq_N
 
   val to_nat : coq_N -> int
 
