src/ocaml/extraction/Decimal.ml
@@ -35,6 +35,21 @@ let rev d =
 
 module Little =
  struct
+  (** val succ : uint -> uint **)
+
+  let rec succ = function
+  | Nil -> D1 Nil
+  | D0 d0 -> D1 d0
+  | D1 d0 -> D2 d0
+  | D2 d0 -> D3 d0
+  | D3 d0 -> D4 d0
+  | D4 d0 -> D5 d0
+  | D5 d0 -> D6 d0
+  | D6 d0 -> D7 d0
+  | D7 d0 -> D8 d0
+  | D8 d0 -> D9 d0
+  | D9 d0 -> D0 (succ d0)
+
   (** val double : uint -> uint **)
 
   let rec double = function
