src/ocaml/extraction/PeanoNat.mli
@@ -1,10 +1,15 @@
 open Datatypes
+open Decimal
 
 module Nat :
  sig
   val pred : int -> int
 
   val compare : int -> int -> comparison
+
+  val to_little_uint : int -> uint -> uint
+
+  val to_uint : int -> uint
 
   val log2_iter : int -> int -> int -> int -> int
 
