src/ocaml/extraction/Strings.mli
@@ -1,0 +1,27 @@
+open BinNat
+open BinNums
+open Decimal
+open DecimalString
+open PeanoNat
+open String0
+
+type signed_int =
+| Pos of uint
+| Neg of uint
+
+val nat_to_signed_int : int -> signed_int
+
+val coq_N_to_signed_int : coq_N -> signed_int
+
+val string_of_signed_int : signed_int -> char list
+
+val string_of_nat : int -> char list
+
+val string_of_N : coq_N -> char list
+
+module type Printer =
+ sig
+  type t
+
+  val to_string : t -> char list
+ end
