src/ocaml/extraction/Var.ml
@@ -5,6 +5,8 @@ open Datatypes
 open FMaps
 open FSets
 open Int0
+open String0
+open Strings
 open ZAriths
 open Eqtype
 
@@ -46,6 +48,18 @@ module VarOrder =
  end
 
 module SSAVarOrder = SsrOrder.MakeProdOrderWithDefaultSucc(VarOrder)(VarOrder)
+
+module SSAVarOrderPrinter =
+ struct
+  type t = SSAVarOrder.t
+
+  (** val to_string : SSAVarOrder.t -> char list **)
+
+  let to_string v =
+    append ('v'::[])
+      (append (string_of_N (fst (Obj.magic v)))
+        (append ('_'::[]) (string_of_N (snd (Obj.magic v)))))
+ end
 
 type ssavar = SSAVarOrder.t
 
