src/ocaml/extraction/Var.mli
@@ -5,6 +5,8 @@ open Datatypes
 open FMaps
 open FSets
 open Int0
+open String0
+open Strings
 open ZAriths
 open Eqtype
 
@@ -67,6 +69,13 @@ module SSAVarOrder :
   val default : t
 
   val succ : t -> t
+ end
+
+module SSAVarOrderPrinter :
+ sig
+  type t = SSAVarOrder.t
+
+  val to_string : SSAVarOrder.t -> char list
  end
 
 type ssavar = SSAVarOrder.t
